zoo_saturn/mpmc_bqueue: WIP.

theories/zoo_saturn/mpmc_bqueue.v
@@ -1,11 +1,24 @@
+From iris.base_logic Require Import
+  lib.ghost_map.
+
 From zoo Require Import
   prelude.
+From zoo.common Require Import
+  countable.
+From zoo.iris.base_logic Require Import
+  lib.mono_list
+  lib.auth_nat_max
+  lib.twins
+  lib.saved_pred.
 From zoo.language Require Import
   notations.
+From zoo.program_logic Require Import
+  typed_prophet.
 From zoo.diaframe Require Import
   diaframe.
 From zoo_std Require Import
-  option.
+  option
+  xtchain.
 From zoo_saturn Require Export
   base
   mpmc_bqueue__code.
@@ -14,37 +27,338 @@ From zoo_saturn Require Import
 From zoo Require Import
   options.
 
+Implicit Types b : bool.
+Implicit Types l front node back new_back : location.
+Implicit Types hist past nodes : list location.
 Implicit Types v t : val.
 Implicit Types vs : list val.
+Implicit Types waiter : gname.
+Implicit Types waiters : gmap gname nat.
+
+#[local] Program Definition prophet := {|
+  typed_strong_prophet1_type :=
+    nat ;
+  typed_strong_prophet1_of_val v _ :=
+    match v with
+    | ValInt i =>
+        Some (Z.to_nat i)
+    | _ =>
+        None
+    end ;
+  typed_strong_prophet1_to_val i :=
+    (#i, ()%V) ;
+|}.
+Solve Obligations of prophet with
+  try done.
+Next Obligation.
+  intros i v _ [= -> ->]. rewrite /= Nat2Z.id //.
+Qed.
 
 Class MpmcBqueueG Σ `{zoo_G : !ZooG Σ} := {
+  #[local] mpmc_bqueue_G_history_G :: MonoListG Σ location ;
+  #[local] mpmc_bqueue_G_front_G :: AuthNatMaxG Σ ;
+  #[local] mpmc_bqueue_G_model_G :: TwinsG Σ (leibnizO (list val)) ;
+  #[local] mpmc_bqueue_G_waiters_G :: ghost_mapG Σ gname nat ;
+  #[local] mpmc_bqueue_G_saved_pred_G :: SavedPredG Σ bool ;
 }.
 
 Definition mpmc_bqueue_Σ := #[
+  mono_list_Σ location ;
+  auth_nat_max_Σ ;
+  twins_Σ (leibnizO (list val)) ;
+  ghost_mapΣ gname nat ;
+  saved_pred_Σ bool
 ].
 #[global] Instance subG_mpmc_bqueue_Σ Σ `{zoo_G : !ZooG Σ} :
   subG mpmc_bqueue_Σ Σ →
   MpmcBqueueG Σ.
 Proof.
+  solve_inG.
 Qed.
 
 Section mpmc_bqueue_G.
   Context `{mpmc_bqueue_G : MpmcBqueueG Σ}.
 
-  Definition mpmc_bqueue_inv t (ι : namespace) (cap : nat) : iProp Σ.
-  Proof. Admitted.
+  Implicit Types Ψ : bool → iProp Σ.
 
-  Definition mpmc_bqueue_model t vs : iProp Σ.
-  Proof. Admitted.
+  Record metadata := {
+    metadata_capacity : nat ;
+    metadata_history : gname ;
+    metadata_front : gname ;
+    metadata_model : gname ;
+    metadata_waiters : gname ;
+  }.
+  Implicit Types γ : metadata.
+
+  #[local] Instance metadata_eq_dec : EqDecision metadata :=
+    ltac:(solve_decision).
+  #[local] Instance metadata_countable :
+    Countable metadata.
+  Proof.
+    solve_countable.
+  Qed.
+
+  #[local] Definition history_auth' γ_history :=
+    mono_list_auth γ_history (DfracOwn 1).
+  #[local] Definition history_auth γ :=
+    history_auth' γ.(metadata_history).
+  #[local] Definition history_at γ :=
+    mono_list_at γ.(metadata_history).
+
+  #[local] Definition front_auth' γ_front :=
+    auth_nat_max_auth γ_front (DfracOwn 1).
+  #[local] Definition front_auth γ :=
+    front_auth' γ.(metadata_front).
+  #[local] Definition front_lb γ :=
+    auth_nat_max_lb γ.(metadata_front).
+
+  #[local] Definition model₁' γ_model vs :=
+    twins_twin1 γ_model (DfracOwn 1) vs.
+  #[local] Definition model₁ γ :=
+    model₁' γ.(metadata_model).
+  #[local] Definition model₂' γ_model vs :=
+    twins_twin2 γ_model vs.
+  #[local] Definition model₂ γ :=
+    model₂' γ.(metadata_model).
+
+  #[local] Definition waiters_auth' γ_waiters :=
+    ghost_map_auth γ_waiters 1.
+  #[local] Definition waiters_auth γ :=
+    waiters_auth' γ.(metadata_waiters).
+  #[local] Definition waiters_at γ waiter :=
+    ghost_map_elem γ.(metadata_waiters) waiter (DfracOwn 1).
+
+  #[local] Definition waiter_au γ ι Ψ : iProp Σ :=
+    AU <{
+      ∃∃ vs,
+      model₁ γ vs
+    }> @ ⊤ ∖ ↑ι, ∅ <{
+      model₁ γ vs
+    , COMM
+      Ψ (bool_decide (vs = []))
+    }>.
+  #[local] Definition waiter_model γ ι past waiter i : iProp Σ :=
+    ∃ Ψ,
+    saved_pred waiter Ψ ∗
+    if decide (i < length past) then
+      Ψ false
+    else
+      waiter_au γ ι Ψ.
+
+  #[local] Definition inv_inner l γ ι : iProp Σ :=
+    ∃ hist past front nodes back vs waiters,
+    ⌜hist = past ++ front :: nodes⌝ ∗
+    ⌜back ∈ hist⌝ ∗
+    l.[front] ↦ #front ∗
+    l.[back] ↦ #back ∗
+    xtchain (Header §Node 4) hist §Null ∗
+    ( [∗ list] node; v ∈ nodes; vs,
+      node.[data] ↦ v
+    ) ∗
+    ( [∗ list] i ↦ node ∈ hist,
+      node.[index] ↦□ #i
+    ) ∗
+    ( [∗ list] i ↦ node ∈ hist,
+      ∃ cap : nat,
+      node.[estimated_capacity] ↦ #cap ∗
+      ⌜i + cap ≤ length past + γ.(metadata_capacity)⌝
+    ) ∗
+    history_auth γ hist ∗
+    front_auth γ (length past) ∗
+    model₂ γ vs ∗
+    waiters_auth γ waiters ∗
+    ( [∗ map] waiter ↦ i ∈ waiters,
+      waiter_model γ ι past waiter i
+    ).
+  #[local] Instance : CustomIpatFormat "inv_inner" :=
+    "(
+      %hist{} &
+      %past{} &
+      %front{} &
+      %nodes{} &
+      %back{} &
+      %vs{} &
+      %waiters{} &
+      >%Hhist{} &
+      >%Hback{} &
+      >Hl_front &
+      >Hl_back &
+      >Hhist &
+      >Hnodes &
+      >Hindices &
+      >Hcapacities &
+      >Hhistory_auth &
+      >Hfront_auth &
+      >Hmodel₂ &
+      >Hwaiters_auth &
+      Hwaiters
+    )".
+  Definition mpmc_bqueue_inv t ι cap : iProp Σ :=
+    ∃ l γ,
+    ⌜t = #l⌝ ∗
+    ⌜cap = γ.(metadata_capacity)⌝ ∗
+    meta l nroot γ ∗
+    l.[capacity] ↦□ #cap ∗
+    inv ι (inv_inner l γ ι).
+  #[local] Instance : CustomIpatFormat "inv" :=
+    "(
+      %l &
+      %γ &
+      -> &
+      -> &
+      #Hmeta &
+      #Hl_capacity &
+      #Hinv
+    )".
+
+  Definition mpmc_bqueue_model t vs : iProp Σ :=
+    ∃ l γ,
+    ⌜t = #l⌝ ∗
+    ⌜length vs ≤ γ.(metadata_capacity)⌝ ∗
+    meta l nroot γ ∗
+    model₁ γ vs.
+  #[local] Instance : CustomIpatFormat "model" :=
+    "(
+      %l_ &
+      %γ_ &
+      %Heq &
+      % &
+      #Hmeta_ &
+      Hmodel₁
+    )".
 
   #[global] Instance mpmc_bqueue_model_timeless t vs :
     Timeless (mpmc_bqueue_model t vs).
   Proof.
-  Admitted.
+    apply _.
+  Qed.
   #[global] Instance mpmc_bqueue_inv_persistent t ι cap :
     Persistent (mpmc_bqueue_inv t ι cap).
   Proof.
-  Admitted.
+    apply _.
+  Qed.
+
+  #[local] Lemma history_alloc front :
+    ⊢ |==>
+      ∃ γ_hist,
+      history_auth' γ_hist [front].
+  Proof.
+    apply mono_list_alloc.
+  Qed.
+  #[local] Lemma history_at_get {γ hist} i node :
+    hist !! i = Some node →
+    history_auth γ hist ⊢
+    history_at γ i node.
+  Proof.
+    apply mono_list_at_get.
+  Qed.
+  #[local] Lemma history_agree γ hist i node :
+    history_auth γ hist -∗
+    history_at γ i node -∗
+    ⌜hist !! i = Some node⌝.
+  Proof.
+    apply mono_list_at_valid.
+  Qed.
+  #[local] Lemma history_update {γ hist} node :
+    history_auth γ hist ⊢ |==>
+    history_auth γ (hist ++ [node]).
+  Proof.
+    apply mono_list_update_snoc.
+  Qed.
+
+  #[local] Lemma front_alloc :
+    ⊢ |==>
+      ∃ γ_front,
+      front_auth' γ_front 0.
+  Proof.
+    apply auth_nat_max_alloc.
+  Qed.
+  #[local] Lemma front_lb_get γ i :
+    front_auth γ i ⊢
+    front_lb γ i.
+  Proof.
+    apply auth_nat_max_lb_get.
+  Qed.
+  #[local] Lemma front_lb_valid γ i1 i2 :
+    front_auth γ i1 -∗
+    front_lb γ i2 -∗
+    ⌜i2 ≤ i1⌝.
+  Proof.
+    apply auth_nat_max_lb_valid.
+  Qed.
+  #[local] Lemma front_update {γ i} i' :
+    i ≤ i' →
+    front_auth γ i ⊢ |==>
+    front_auth γ i'.
+  Proof.
+    apply auth_nat_max_update.
+  Qed.
+
+  #[local] Lemma model_alloc :
+    ⊢ |==>
+      ∃ γ_model,
+      model₁' γ_model [] ∗
+      model₂' γ_model [].
+  Proof.
+    apply twins_alloc'.
+  Qed.
+  #[local] Lemma model_agree γ vs1 vs2 :
+    model₁ γ vs1 -∗
+    model₂ γ vs2 -∗
+    ⌜vs1 = vs2⌝.
+  Proof.
+    apply: twins_agree_L.
+  Qed.
+  #[local] Lemma model_update {γ vs1 vs2} vs :
+    model₁ γ vs1 -∗
+    model₂ γ vs2 ==∗
+      model₁ γ vs ∗
+      model₂ γ vs.
+  Proof.
+    apply twins_update'.
+  Qed.
+
+  #[local] Lemma waiters_alloc :
+    ⊢ |==>
+      ∃ γ_waiters,
+      waiters_auth' γ_waiters ∅.
+  Proof.
+    iMod ghost_map_alloc as "(%γ_waiters & Hwaiters_auth & _)".
+    iSteps.
+  Qed.
+  #[local] Lemma waiters_lookup γ waiters waiter i :
+    waiters_auth γ waiters -∗
+    waiters_at γ waiter i -∗
+    ⌜waiters !! waiter = Some i⌝.
+  Proof.
+    apply ghost_map_lookup.
+  Qed.
+  #[local] Lemma waiters_insert {γ waiters} waiter i :
+    waiters !! waiter = None →
+    waiters_auth γ waiters ⊢ |==>
+      waiters_auth γ (<[waiter := i]> waiters) ∗
+      waiters_at γ waiter i.
+  Proof.
+    iIntros "%Hlookup Hwaiters_auth".
+    iApply (ghost_map_insert with "Hwaiters_auth"); first done.
+  Qed.
+  #[local] Lemma waiters_delete γ waiters waiter i :
+    waiters_auth γ waiters -∗
+    waiters_at γ waiter i ==∗
+    waiters_auth γ (delete waiter waiters).
+  Proof.
+    apply ghost_map_delete.
+  Qed.
+
+  Lemma mpmc_bqueue_model_valid t ι cap vs :
+    mpmc_bqueue_inv t ι cap -∗
+    mpmc_bqueue_model t vs -∗
+    ⌜length vs ≤ cap⌝.
+  Proof.
+    iIntros "(:inv) (:model)". injection Heq as <-.
+    iDestruct (meta_agree with "Hmeta Hmeta_") as %<-. iClear "Hmeta_".
+    iSteps.
+  Qed.
 
   Lemma mpmc_bqueue_create_spec ι cap :
     (0 ≤ cap)%Z →
@@ -58,7 +372,39 @@ Section mpmc_bqueue_G.
       mpmc_bqueue_model t []
     }}}.
   Proof.
-  Admitted.
+    iIntros "%Hcap %Φ _ HΦ".
+
+    wp_rec.
+
+    wp_block front as "Hfront_header" "_" "(Hfront_next & Hfront_data & Hfront_index & Hfront_capacity & _)".
+    iMod (pointsto_persist with "Hfront_index") as "#Hfront_index".
+    wp_block l as "Hmeta" "(Hl_capacity & Hl_front & Hl_back & _)".
+    iMod (pointsto_persist with "Hl_capacity") as "#Hcapacity".
+
+    iMod history_alloc as "(%γ_history & Hhistory_auth)".
+    iMod front_alloc as "(%γ_front & Hfront_auth)".
+    iMod model_alloc as "(%γ_model & Hmodel₁ & Hmodel₂)".
+    iMod waiters_alloc as "(%γ_waiters & Hwaiters_auth)".
+
+    pose γ := {|
+      metadata_capacity := ₊cap ;
+      metadata_history := γ_history ;
+      metadata_front := γ_front ;
+      metadata_model := γ_model ;
+      metadata_waiters := γ_waiters ;
+    |}.
+
+    iMod (meta_set _ _ γ with "Hmeta") as "#Hmeta"; first done.
+
+    iApply "HΦ".
+    iSplitR "Hmodel₁"; last iSteps.
+    iExists l, γ. rewrite Z2Nat.id //. iStep 4.
+    iApply inv_alloc.
+    iExists [front], [], front, [], front, [], ∅. iFrameSteps.
+    { rewrite elem_of_list_singleton //. }
+    rewrite xtchain_singleton. iSteps.
+    rewrite big_sepM_empty //.
+  Qed.
 
   Lemma mpmc_bqueue_capacity_spec t ι cap :
     {{{
@@ -70,7 +416,84 @@ Section mpmc_bqueue_G.
       True
     }}}.
   Proof.
-  Admitted.
+    iSteps.
+  Qed.
+
+  #[local] Lemma front_spec_strong au Ψ l γ ι :
+    {{{
+      inv ι (inv_inner l γ ι) ∗
+      if negb au then True else
+        waiter_au γ ι Ψ
+    }}}
+      (#l).{front}
+    {{{ front i,
+      RET #front;
+      history_at γ i front ∗
+      front.[index] ↦□ #i ∗
+      front_lb γ i ∗
+      if negb au then True else
+        ∃ waiter,
+        saved_pred waiter Ψ ∗
+        waiters_at γ waiter i
+    }}}.
+  Proof.
+    iIntros "%Φ (#Hinv & HΨ) HΦ".
+
+    iInv "Hinv" as "(:inv_inner)".
+    wp_load.
+    assert (hist !! length past = Some front) as Hhist_lookup.
+    { rewrite Hhist list_lookup_middle //. }
+    iDestruct (history_at_get _ front with "Hhistory_auth") as "#Hhistory_at"; first done.
+    iDestruct (big_sepL_lookup with "Hindices") as "#Hfront_index"; first done.
+    iDestruct (front_lb_get with "Hfront_auth") as "#Hfront_lb".
+    destruct au; last iSteps.
+    iMod (saved_pred_alloc_cofinite (dom waiters) Ψ) as "(%waiter & %Hwaiter & #Hwaiter)".
+    rewrite not_elem_of_dom in Hwaiter.
+    iMod (waiters_insert _ (length past) with "Hwaiters_auth") as "(Hwaiter_auth & Hwaiters_at)"; first done.
+    iDestruct (big_sepM_insert_2 _ _ waiter (length past) with "[HΨ] Hwaiters") as "Hwaiters".
+    { iExists Ψ. rewrite decide_False; first lia. iSteps. }
+    iSplitR "Hwaiters_at HΦ". { iFrameSteps. }
+    iSteps.
+  Qed.
+  #[local] Lemma front_spec l γ ι :
+    {{{
+      inv ι (inv_inner l γ ι)
+    }}}
+      (#l).{front}
+    {{{ front i,
+      RET #front;
+      history_at γ i front ∗
+      front.[index] ↦□ #i ∗
+      front_lb γ i
+    }}}.
+  Proof.
+    iIntros "%Φ #Hinv HΦ".
+    wp_apply (front_spec_strong false inhabitant with "[$Hinv]").
+    iSteps.
+  Qed.
+
+  #[local] Lemma back_spec l γ ι :
+    {{{
+      inv ι (inv_inner l γ ι)
+    }}}
+      (#l).{back}
+    {{{ back i,
+      RET #back;
+      history_at γ i back ∗
+      back.[index] ↦□ #i
+    }}}.
+  Proof.
+    iIntros "%Φ #Hinv HΦ".
+
+    iInv "Hinv" as "(:inv_inner)".
+    wp_load.
+    pose proof Hback as (i & Hlookup)%elem_of_list_lookup.
+    iDestruct (history_at_get with "Hhistory_auth") as "#Hhistory_elem_back"; first done.
+    iAssert (back.[index] ↦□ #i)%I as "#Hback_index".
+    { rewrite big_sepL_lookup //. }
+    iSplitR "HΦ". { iFrameSteps. }
+    iSteps.
+  Qed.
 
   Lemma mpmc_bqueue_size_spec t ι cap :
     <<<
